@prefix rdf:    <http://www.w3.org/1999/02/22-rdf-syntax-ns#> .
@prefix rdfs:   <http://www.w3.org/2000/01/rdf-schema#> .
@prefix owl:    <http://www.w3.org/2002/07/owl#> .
@prefix cc:     <http://creativecommons.org/ns#> .
@prefix xsd:    <http://www.w3.org/2001/XMLSchema#> .
@prefix mv:     <http://schema.mobivoc.org/> .
@prefix gr:     <http://purl.org/goodrelations/v1#> .
@prefix dbo:    <http://dbpedia.org/ontology/> .
@prefix dct:    <http://purl.org/dc/terms/> .
@prefix vann:   <http://purl.org/vocab/vann/> .
@prefix foaf:   <http://xmlns.com/foaf/0.1/> .
@prefix vs:     <http://www.w3.org/2003/06/sw-vocab-status/ns#> .
@prefix schema: <http://schema.org/> .
@prefix vp:     <https://velopark.ilabt.imec.be/openvelopark/vocabulary#> .
@prefix vpt:    <https://velopark.ilabt.imec.be/openvelopark/terms#> .


vp:     a                 foaf:Document ;
        foaf:primaryTopic vp: ;
        dct:issued        "2019-01-29"^^xsd:date ;
        dct:modified      "2019-11-26"^^xsd:date ;
        dct:hasFormat     vp: ;
        cc:license        <https://creativecommons.org/licenses/by/4.0/> ;
        dct:rights        "Copyright 2019 - Open Velopark contributors" .

vp:     a                 owl:Ontology ;
        rdfs:label        "Open Velopark Vocabulary"@en ;
        dct:description   "This ontology introduces the definition of a set of bicycle parking facilities related terms. It reuses and extends the MobiVoc (see http://schema.mobivoc.org/) and the schema.org (see https://schema.org) vocabularies."@en ;
        vann:preferredNamespacePrefix  "openvelopark" ;
        vann:preferredNamespaceUri     "https://velopark.ilabt.imec.be/openvelopark/vocabulary";
        rdfs:seeAlso      mv:, schema:, vpt: ;
        rdfs:seeAlso      <https://www.velopark.be/> ;
        dct:creator       <https://biblio.ugent.be/person/802002620753> ;
        dct:creator       <https://pietercolpaert.be/#me> .
        #owl:imports       schema:, mv:, vpt: .

<https://biblio.ugent.be/person/802002620753> 
        a                 foaf:Person, schema:Person ;
        foaf:name         "Julian Rojas" ;
        foaf:mbox         "julianandres.rojasmelendez@ugent.be" .
        

#################################################################
#
#    Classes
#
#################################################################

vp:Bicycle  
        a                 rdfs:Class , owl:Class ;
        rdfs:comment      "A single-track vehicle, having two wheels attached to a frame, one behind the other."@en ;
        rdfs:isDefinedBy  vp: ;
        rdfs:label        "Bicycle"@en ;
        rdfs:subClassOf   schema:Vehicle ;
        dct:created       "2019-01-29"^^xsd:date ;
        dct:modified      "2019-01-29"^^xsd:date ;
        vs:term_status    "stable" .

vp:BikeParkingFeature 
        a                 rdfs:Class , owl:Class ;
        rdfs:comment      "A feature available for a given parking facility."@en ;
        rdfs:isDefinedBy  vp: ;
        rdfs:label        "Bike Parking Feature"@en ;
        rdfs:subClassOf   schema:LocationFeatureSpecification ;
        dct:created       "2019-01-29"^^xsd:date ;
        dct:modified      "2019-01-29"^^xsd:date ;
        vs:term_status    "stable" .

vp:SecurityFeature 
        a                 rdfs:Class , owl:Class ;
        rdfs:comment      "A security feature available for a given location or facility."@en ;
        rdfs:isDefinedBy  vp: ;
        rdfs:label        "Security Feature"@en ;
        rdfs:subClassOf   schema:LocationFeatureSpecification ;
        dct:created       "2019-05-20"^^xsd:date ;
        dct:modified      "2019-05-20"^^xsd:date ;
        vs:term_status    "stable" .

vp:AllowedBicycle  
        a                 rdfs:Class , owl:Class ;
        rdfs:comment      "A bicycle that is allowed in a given parking facility." ;
        rdfs:isDefinedBy  vp: ;
        rdfs:label        "Allowed Bicycle"@en ;
        dct:created       "2019-01-29"^^xsd:date ;
        dct:modified      "2019-01-29"^^xsd:date ;
        vs:term_status    "stable" .


#################################################################
#
#    Object Properties
#
#################################################################

vp:dataOwner  
        a                 rdf:Property , owl:ObjectProperty ;
        rdfs:comment      "The owner of the data about a certain bicycle parking facility."@en ;
        rdfs:domain       mv:BicycleParkingStation ;
        rdfs:isDefinedBy  vp: ;
        rdfs:label        "data owner"@en ;
        rdfs:range        gr:BusinessEntity ;
        dct:created       "2019-01-30"^^xsd:date ;
        dct:modified      "2019-01-30"^^xsd:date ;
        vs:term_status    "stable" .

vp:allows  
        a                 rdf:Property , owl:ObjectProperty ;
        rdfs:comment      "Indicates a type of bicycle that is allowed in a certain parking facility."@en ;
        rdfs:domain       mv:BicycleParkingStation ;
        rdfs:isDefinedBy  vp: ;
        rdfs:label        "allows"@en ;
        rdfs:range        vp:AllowedBicycle ;
        dct:created       "2019-01-30"^^xsd:date ;
        dct:modified      "2019-01-30"^^xsd:date ;
        vs:term_status    "stable" .

vp:bicycleType  
        a                 rdf:Property , owl:ObjectProperty ;
        rdfs:comment      "Indicates the specific type of bicycle that is allowed in a certain parking facility."@en ;
        rdfs:domain       vp:AllowedBicycle ;
        rdfs:isDefinedBy  vp: ;
        rdfs:label        "bicycle type"@en ;
        rdfs:range        vp:Bicycle ;
        dct:created       "2019-01-30"^^xsd:date ;
        dct:modified      "2019-01-30"^^xsd:date ;
        vs:term_status    "stable" .


#################################################################
#
#    Data properties
#
#################################################################

vp:startDate
        a                 owl:DatatypeProperty , rdf:Property ;
        rdfs:comment      "The initial opening date of a parking facility (in ISO 8601 date format)."@en ;
        rdfs:domain       mv:BicycleParkingStation ;
        rdfs:isDefinedBy  vp: ;
        rdfs:label        "start date"@en ;
        rdfs:range        xsd:date .

vp:endDate
        a                 owl:DatatypeProperty , rdf:Property ;
        rdfs:comment      "The final closing date of a parking facility (in ISO 8601 date format)."@en ;
        rdfs:domain       mv:BicycleParkingStation ;
        rdfs:isDefinedBy  vp: ;
        rdfs:label        "end date"@en ;
        rdfs:range        xsd:date .

vp:minimumStorageTime  
        a                 rdf:Property , owl:DatatypeProperty ;
        rdfs:comment      "Indicates the minimum amount of time that bicycles are allowed to be parked in a certain parking facility."@en ;
        rdfs:domain       mv:BicycleParkingStation ;
        rdfs:isDefinedBy  vp: ;
        rdfs:label        "minimum storage time"@en ;
        rdfs:range        xsd:duration ;
        dct:created       "2019-01-30"^^xsd:date ;
        dct:modified      "2019-01-30"^^xsd:date ;
        vs:term_status    "stable" .

vp:maximumParkingDuration  
        a                 rdf:Property , owl:DatatypeProperty ;
        rdfs:comment      "Indicates the maximum amount of time that bicycles are allowed to be parked in a certain parking facility."@en ;
        rdfs:domain       mv:BicycleParkingStation ;
        rdfs:isDefinedBy  vp: ;
        rdfs:label        "maximum parking duration"@en ;
        rdfs:range        xsd:duration ;
        dct:created       "2019-01-30"^^xsd:date ;
        dct:modified      "2019-01-30"^^xsd:date ;
        vs:term_status    "stable" .

vp:intendedAudience  
        a                 rdf:Property , owl:DatatypeProperty ;
        rdfs:comment      "Indicates the type of audience that can make use of a certain parking facility."@en ;
        rdfs:domain       mv:BicycleParkingStation ;
        rdfs:isDefinedBy  vp: ;
        rdfs:label        "intended audience"@en ;
        rdfs:range        xsd:string ;
        dct:created       "2019-01-30"^^xsd:date ;
        dct:modified      "2019-01-30"^^xsd:date ;
        vs:term_status    "stable" .

vp:restrictions  
        a                 rdf:Property , owl:DatatypeProperty ;
        rdfs:comment      "Indicates the operational restrictions that a certain parking facility may have."@en ;
        rdfs:domain       mv:BicycleParkingStation ;
        rdfs:isDefinedBy  vp: ;
        rdfs:label        "restrictions"@en ;
        rdfs:range        xsd:string ;
        dct:created       "2019-01-30"^^xsd:date ;
        dct:modified      "2019-01-30"^^xsd:date ;
        vs:term_status    "stable" .

vp:removalConditions  
        a                 rdf:Property , owl:DatatypeProperty ;
        rdfs:comment      "Description of the conditions under which a bicycle may be removed from a certain parking facility."@en ;
        rdfs:domain       mv:BicycleParkingStation ;
        rdfs:isDefinedBy  vp: ;
        rdfs:label        "removal conditions"@en ;
        rdfs:range        xsd:string ;
        dct:created       "2019-01-30"^^xsd:date ;
        dct:modified      "2019-01-30"^^xsd:date ;
        vs:term_status    "stable" .

vp:postRemovalAction  
        a                 rdf:Property , owl:DatatypeProperty ;
        rdfs:comment      "Description of how parking facility users must proceed when their bicycles are removed."@en ;
        rdfs:domain       mv:BicycleParkingStation ;
        rdfs:isDefinedBy  vp: ;
        rdfs:label        "post removal action"@en ;
        rdfs:range        xsd:string ;
        dct:created       "2019-01-30"^^xsd:date ;
        dct:modified      "2019-01-30"^^xsd:date ;
        vs:term_status    "stable" .

vp:bicyclesAmount  
        a                 rdf:Property , owl:DatatypeProperty ;
        rdfs:comment      "Indicates the maximum amount of bicycle of a certain type that are allowed in a parking facility."@en ;
        rdfs:domain       vp:AllowedBicycle ;
        rdfs:isDefinedBy  vp: ;
        rdfs:label        "bicycles amount"@en ;
        rdfs:range        xsd:integer ;
        dct:created       "2019-01-30"^^xsd:date ;
        dct:modified      "2019-01-30"^^xsd:date ;
        vs:term_status    "stable" .

vp:countingSystem  
        a                 rdf:Property , owl:DatatypeProperty ;
        rdfs:comment      "Indicates whether a certain type of allowed bicycle has a counting system or not, for a given parking facility."@en ;
        rdfs:domain       vp:AllowedBicycle ;
        rdfs:isDefinedBy  vp: ;
        rdfs:label        "counting system"@en ;
        rdfs:range        xsd:boolean ;
        dct:created       "2019-01-30"^^xsd:date ;
        dct:modified      "2019-01-30"^^xsd:date ;
        vs:term_status    "stable" .


#################################################################
#
#    Individuals
#
#################################################################

vpt:PublicBicycleParking  
        a                 mv:BicycleParkingStation ;
        rdfs:comment      "Bicycle parking facility available for public use."@en, 
                          "Fietsenstalling beschikbaar voor openbaar gebruik."@nl, 
                          "Stationnement pour vélos disponible pour un usage public."@fr, 
                          "Fahrradabstellplatz zur öffentlichen Nutzung."@de ;
        rdfs:isDefinedBy  vpt: ;
        rdfs:label        "Public Bicycle Parking"@en, "Openbare Fietsenstalling"@nl, "Parking Vélo Public"@fr, "Öffentlicher Fahrradabstellplatz"@de ;
        dct:created       "2019-05-20"^^xsd:date ;
        dct:modified      "2019-05-20"^^xsd:date ;
        vs:term_status    "stable" .

vpt:ResidentBicycleParking  
        a                 mv:BicycleParkingStation ;
        rdfs:comment      "Bicycle parking in the specifically designed space of a building, only accessible to local residents."@en, 
                          "Stalling in specifiek daarvoor ingerichte ruimte van een gebouw, enkel toegankelijk voor omwonenden uit de buurt."@nl, 
                          "Stockage dans l'espace spécialement conçu d'un bâtiment, accessible uniquement aux résidents locaux."@fr, 
                          "Lagerung im speziell gestalteten Raum eines Gebäudes, nur für Anwohner zugänglich."@de ;
        rdfs:isDefinedBy  vpt: ;
        rdfs:label        "Resident Bicycle Parking"@en, "Buurtstalling"@nl, "Parking Vélo Riverains"@fr, "Resident Fahrradabstellplatz"@de ;
        dct:created       "2019-01-29"^^xsd:date ;
        dct:modified      "2019-11-25"^^xsd:date ;
        vs:term_status    "stable" .

vpt:BicycleLocker  
        a                 mv:BicycleParkingStation ;
        rdfs:comment      "Covered and lockable bicycle parking facility on public roads."@en, 
                          "Overdekte en afsluitbare fietsenstalling op openbare wegen."@nl, 
                          "Parking vélo couvert et verrouillable sur la voie publique."@fr, 
                          "Überdachter und abschließbarer Fahrradabstellplatz auf öffentlichen Straßen."@de ;
        rdfs:isDefinedBy  vpt: ;
        rdfs:label        "Bicycle Locker"@en, "Fietskluis"@nl, "Casier de Bicyclette"@fr, "Fahrradschrank"@de ;
        dct:created       "2019-01-29"^^xsd:date ;
        dct:modified      "2019-05-20"^^xsd:date ;
        vs:term_status    "stable" .

vpt:BicycleStand  
        a                 mv:BicycleParkingStation ;
        rdfs:comment      "Device to which bicycles can be securely attached for parking purposes."@en, 
                          "Apparaat waaraan fietsen veilig kunnen worden bevestigd voor parkeren."@nl, 
                          "Dispositif auquel des bicyclettes peuvent être solidement attachées à des fins de stationnement."@fr, 
                          "Gerät, an dem Fahrräder zum Parken sicher befestigt werden können."@de ;
        rdfs:isDefinedBy  vpt: ;
        rdfs:label        "Bicycle Stand"@en, "Fietsbeugel"@nl, "Support de Vélo"@fr, "Fahrradständer"@de ;
        dct:created       "2019-11-25"^^xsd:date ;
        dct:modified      "2019-11-25"^^xsd:date ;
        vs:term_status    "stable" .

vpt:RegularBicycle  
        a                 vp:Bicycle ;
        rdfs:comment      "A regular bicycle that does not have any special features."@en, 
                          "Een gewone fiets die geen speciale functies heeft."@nl, 
                          "Un vélo ordinaire qui ne présente aucune particularité."@fr, 
                          "Ein normales Fahrrad, das keine Besonderheiten aufweist."@de ;
        rdfs:isDefinedBy  vpt: ;
        rdfs:label        "Regular Bicycle"@en, "Normale Fiets"@nl, "Vélo Classique"@fr, "Normales Fahrrad"@de ;
        dct:created       "2019-01-29"^^xsd:date ;
        dct:modified      "2019-05-20"^^xsd:date ;
        vs:term_status    "stable" .

vpt:ElectricBicycle  
        a                 vp:Bicycle ;
        rdfs:comment      "An electrically powered bicycle."@en, 
                          "Een elektrisch aangedreven fiets."@nl, 
                          "Un vélo à propulsion électrique."@fr, 
                          "Ein elektrisch angetriebenes Fahrrad."@de ;
        rdfs:isDefinedBy  vpt: ;
        rdfs:label        "Electric Bicycle"@en, "Elektrische Fiets"@nl, "Vélo Électrique"@fr, "Elektrofahrrad"@de ;
        dct:created       "2019-01-29"^^xsd:date ;
        dct:modified      "2019-05-20"^^xsd:date ;
        vs:term_status    "stable" .

vpt:CargoBicycle  
        a                 vp:Bicycle ;
        rdfs:comment      "A bicycle specially adapted to transport load."@en, 
                          "Een speciaal aangepaste fiets om lading te vervoeren."@nl, 
                          "Un vélo spécialement adapté au transport de charge."@fr, 
                          "Ein Fahrrad, das speziell für den Transport von Lasten ausgelegt ist."@de ;
        rdfs:isDefinedBy  vpt: ;
        rdfs:label        "Cargo Bicycle"@en, "Bakfiets"@nl, "Vélo Cargo"@fr, "Lastenfahrrad"@de ;
        dct:created       "2019-01-29"^^xsd:date ;
        dct:modified      "2019-05-20"^^xsd:date ;
        vs:term_status    "stable" .

vpt:TandemBicycle  
        a                 vp:Bicycle ;
        rdfs:comment      "A bicycle designed to be ridden by more than one person."@en, 
                          "Een fiets die ontworpen is om door meer dan één persoon te worden bereden."@nl, 
                          "Un vélo conçu pour être monté par plus d'une personne."@fr, 
                          "Ein Fahrrad, das von mehr als einer Person gefahren werden kann."@de ;
        rdfs:isDefinedBy  vpt: ;
        rdfs:label        "Tandem Bicycle"@en, "Tandemfiets"@nl, "Vélo Tandem"@fr, "Tandemfahrrad"@de ;
        dct:created       "2019-01-29"^^xsd:date ;
        dct:modified      "2019-05-20"^^xsd:date ;
        vs:term_status    "stable" .

vpt:CameraSurveillance  
        a                 vp:SecurityFeature ;
        rdfs:comment      "A facility feature that indicates it has surveillance cameras available."@en, 
                          "Een faciliteitsfunctie die aangeeft dat er bewakingscamera's beschikbaar zijn."@nl, 
                          "Une fonctionnalité qui indique que des caméras de surveillance sont disponibles."@fr, 
                          "Eine Funktion, die anzeigt, dass Überwachungskameras verfügbar sind."@de ;
        rdfs:isDefinedBy  vpt: ;
        rdfs:label        "Camera Surveillance"@en, "Camerabewaking"@nl, "Surveillance par Caméra"@fr, "Kameraüberwachung"@de ;
        dct:created       "2019-01-29"^^xsd:date ;
        dct:modified      "2019-11-25"^^xsd:date ;
        vs:term_status    "stable" .

vpt:PersonnelSupervision 
        a                 vp:SecurityFeature ;
        rdfs:comment      "A facility feature that indicates it has personnel supervision available."@en, 
                          "Een faciliteitsfunctie die aangeeft dat er personeelsbewaking beschikbaar is."@nl, 
                          "Une fonctionnalité qui indique qu’une supervision du personnel est disponible."@fr, 
                          "Eine Einrichtungsfunktion, die angibt, dass eine Personalüberwachung verfügbar ist."@de ;
        rdfs:isDefinedBy  vpt: ;
        rdfs:label        "Personnel Supervision"@en, "Beveiligingspersoneel"@nl, "Personnel de Sécurité"@fr, "Sicherheitspersonal"@de ;
        dct:created       "2019-01-29"^^xsd:date ;
        dct:modified      "2019-05-20"^^xsd:date ;
        vs:term_status    "stable" .

vpt:ElectronicAccess  
        a                 vp:SecurityFeature ;
        rdfs:comment      "A facility feature that indicates it has an electronic access system."@en, 
                          "Een faciliteitsfunctie die aangeeft dat het een elektronisch toegangssysteem heeft."@nl, 
                          "Une fonctionnalité qui indique qu’il dispose d’un système d’accès électronique."@fr, 
                          "Ein Funktionsmerkmal, das angibt, dass es über ein elektronisches Zugangssystem verfügt."@de ;
        rdfs:isDefinedBy  vpt: ;
        rdfs:label        "Electronic Access"@en, "Elektronische Toegang"@nl, "Contrôle d'Accès Électronique"@fr, "Elektronischer Zugang"@de ;
        dct:created       "2019-01-29"^^xsd:date ;
        dct:modified      "2019-05-20"^^xsd:date ;
        vs:term_status    "stable" .

vpt:LockerService 
        a                 vp:SecurityFeature ;
        rdfs:comment      "A facility feature that indicates it has a locker service available."@en, 
                          "Een faciliteitsfunctie die aangeeft dat er een lockerservice beschikbaar is."@nl, 
                          "Une fonctionnalité qui indique qu’un service de casier est disponible."@fr, 
                          "Eine Einrichtungsfunktion, die angibt, dass ein Schließfachdienst verfügbar ist."@de ;
        rdfs:isDefinedBy  vpt: ;
        rdfs:label        "Locker Service"@en, "Lockerservice"@nl, "Service de Casier"@fr, "Schließfachservice"@de ;
        dct:created       "2019-01-29"^^xsd:date ;
        dct:modified      "2019-05-20"^^xsd:date ;
        vs:term_status    "stable" .

vpt:BicyclePump  
        a                 vp:BikeParkingFeature ;
        rdfs:comment      "A parking facility feature that indicates it has a bicycle pump available."@en, 
                          "Een parkeerfaciliteit die aangeeft dat er een fietspomp beschikbaar is."@nl, 
                          "Une fonctionnalité de parking indiquant qu’une pompe à vélo est disponible."@fr, 
                          "Eine Parkfunktion, die anzeigt, dass eine Fahrradpumpe verfügbar ist."@de ;
        rdfs:isDefinedBy  vpt: ;
        rdfs:label        "Bicycle Pump"@en, "Fietspomp"@nl, "Pompe à Vélo"@fr, "Fahrradpumpe"@de ;
        dct:created       "2019-01-29"^^xsd:date ;
        dct:modified      "2019-05-20"^^xsd:date ;
        vs:term_status    "stable" .

vpt:MaintenanceService 
        a                 vp:BikeParkingFeature ;
        rdfs:comment      "A parking facility feature that indicates it has a bicycle maintenance service available."@en, 
                          "Een parkeerfaciliteit die aangeeft dat er een fietsonderhoudsdienst beschikbaar is."@nl, 
                          "Une fonctionnalité de parking indiquant qu’un service d’entretien des vélos est disponible."@fr, 
                          "Eine Parkfunktion, die anzeigt, dass ein Fahrradwartungsservice verfügbar ist."@de ;
        rdfs:isDefinedBy  vpt: ;
        rdfs:label        "Maintenance Service"@en, "Onderhoudsdienst"@nl, "Service de Maintenance"@fr, "Wartungsservice"@de ;
        dct:created       "2019-01-29"^^xsd:date ;
        dct:modified      "2019-01-29"^^xsd:date ;
        vs:term_status    "stable" .

vpt:ChargingPoint 
        a                 vp:BikeParkingFeature ;
        rdfs:comment      "A parking facility feature that indicates it has an electrical bicycle charging point available."@en, 
                          "Een parkeervoorziening die aangeeft dat er een elektrisch fietslaadpunt beschikbaar is."@nl, 
                          "Une fonction de parcage indiquant qu’il dispose d’un point de charge pour vélo électrique."@fr, 
                          "Eine Parkfunktion, die anzeigt, dass eine Ladestation für Elektrofahrräder verfügbar ist."@de ;
        rdfs:isDefinedBy  vpt: ;
        rdfs:label        "Charging Point"@en, "Oplaadpunt"@nl, "Borne de Recharge"@fr, "Ladepunkt"@de ;
        dct:created       "2019-01-29"^^xsd:date ;
        dct:modified      "2019-05-20"^^xsd:date ;
        vs:term_status    "stable" .

vpt:ToiletService 
        a                 vp:BikeParkingFeature ;
        rdfs:comment      "A parking facility feature that indicates it has a toilet service available."@en, 
                          "Een parkeerfaciliteit die aangeeft dat er een toiletservice beschikbaar is."@nl, 
                          "Une fonctionnalité de parking qui indique qu'il a un service de toilette disponible."@fr, 
                          "Eine Parkmöglichkeit, die anzeigt, dass ein Toilettenservice verfügbar ist."@de ;
        rdfs:isDefinedBy  vpt: ;
        rdfs:label        "Toilet Service"@en, "Toiletten"@nl, "Toilettes"@fr, "Toilettenservice"@de ;
        dct:created       "2019-01-29"^^xsd:date ;
        dct:modified      "2019-05-20"^^xsd:date ;
        vs:term_status    "stable" .

vpt:BikeRentalService 
        a                 vp:BikeParkingFeature ;
        rdfs:comment      "A parking facility feature that indicates it has a bicycle rental service available."@en, 
                          "Een parkeerfaciliteit die aangeeft dat er een fietsverhuur beschikbaar is."@nl, 
                          "Un parking qui indique qu’un service de location de vélos est disponible."@fr, 
                          "Eine Parkmöglichkeit, die anzeigt, dass ein Fahrradverleih zur Verfügung steht."@de ;
        rdfs:isDefinedBy  vpt: ;
        rdfs:label        "Bike Rental Service"@en, "Fietsverhuur"@nl, "Service de Location de Vélos"@fr, "Fahrradverleih"@de ;
        dct:created       "2019-01-29"^^xsd:date ;
        dct:modified      "2019-05-20"^^xsd:date ;
        vs:term_status    "stable" .

vpt:BikeSharing 
        a                 vp:BikeParkingFeature ;
        rdfs:comment      "A service in which bicycles are made available for shared use to individuals on a short term basis."@en, 
                          "Een service waarbij fietsen op korte termijn beschikbaar worden gesteld voor gedeeld gebruik aan particulieren."@nl, 
                          "Un service dans lequel des vélos sont mis à la disposition des particuliers pour une utilisation partagée à court terme."@fr, 
                          "Ein Service, bei dem Fahrräder für Einzelpersonen kurzfristig zur gemeinsamen Nutzung zur Verfügung gestellt werden."@de ;
        rdfs:isDefinedBy  vpt: ;
        rdfs:label        "Bike Sharing"@en, "Deelfiets"@nl, "Vélos en Libre Partage"@fr, "Fahrard Teilen"@de ;
        dct:created       "2019-11-26"^^xsd:date ;
        dct:modified      "2019-11-26"^^xsd:date ;
        vs:term_status    "stable" .